* Exercise 1.13

In our example, we began by eliminating the Kleene star in the grammar
for =S-list=. Write =subst= following the original grammar by using
=map=.

** Answer
 Recall the grammar:

#+BEGIN_SRC
S-list ::= ( {S-exp}* )
S-exp  ::= Symbol | S-list
#+END_SRC

Then,

#+BEGIN_SRC racket
(define subst
  (lambda (new old slist)
    (map (lambda (sexp)
         (if (symbol? sexp)
             (if (eqv? sexp old) new sexp)
             (subst new old sexp)))
       slist)))
#+END_SRC

(Thank you, SICP)
