* Exercise 1.14

Given the assumption =0 â‰¤ n < length(v)=, prove that
=partial-vector-sum= is correct.

** Answer
We can prove it (as per the book's suggestion) via induction.

Let the induction hypothesis =IH(k)= be that =partial-vector-sum k= is
the sum of the =kth= first elements in the vector. We must prove that
=IH(0)= holds and that, given that =IH(k)= holds, that =IH(k + 1)= holds
too.

=IH(0)= holds because =partial-vector-sum 0= yields =v(0)=, which is
indeed the sum from the 0th element to the 0th element. =IH(k + 1)=
holds because =IH(k + 1) = IH(k) + v(k + 1)= and =IH(k)= holds.

In other words, =partial-vector-sum (k + 1)= is the sum from =0= to =k=
plus =v(k + 1)=, which is equal to the sum from =0= to =k + 1=, which
is what we wanted to prove.
